experiments/coq-experiments/proplang/OptionalOverhead/Collect.py
@@ -8,23 +8,20 @@ from benchtool.Tasks import tasks
 def collect(results: str):
     tool = Coq(results=results, replace_level=ReplaceLevel.REPLACE, log_level=LogLevel.DEBUG)
 
-    common = tool.common()
-
-    variables = list(filter(lambda v: v.name == "Energy-v1", tool.all_variables(common)))
-    mixtures = tool.all_variable_mixtures(variables)
-
     for workload in tool.all_workloads():
         if not workload.name.endswith('Proplang'):
             continue
 
         tool._preprocess(workload)
 
+        variables = list(filter(lambda v: v.name == "PropLangVersion", tool.all_variables(workload)))
+        mixtures = tool.all_variable_mixtures(variables)
 
         for mixture in mixtures:
             print("Mixture")
             for variable, version  in mixture:
                 print(f"Applying Variable {variable}::{version}")
-                tool.update_variable(common, variable, version)
+                tool.update_variable(workload, variable, version)
 
             for variant in tool.all_variants(workload):
 
@@ -34,7 +31,7 @@ def collect(results: str):
                 run_trial = None
 
                 for strategy in tool.all_strategies(workload):
-                    if not strategy.name.endswith('Fuzzer'):
+                    if not strategy.name.startswith('Spec'):
                         continue
 
                     for property in tool.all_properties(workload):
@@ -65,8 +62,8 @@ def collect(results: str):
                                             strategy=strategy.name,
                                             property=property,
                                             file=file,
-                                            trials=10,
-                                            timeout=60,
+                                            trials=50,
+                                            timeout=10,
                                             short_circuit=True)
                         run_trial(cfg)
 
