experiments/coq-experiments/proplang/OptionalOverhead/notes.md
@@ -2,3 +2,6 @@
 **Experiment Commit:**
 
 **Description:** 
+
+Trials: 50
+Time Bound: 10 seconds
